src/Spec/Protocol.v
@@ -1,12 +1,55 @@
 Require Import ConcurProc.
 Require Import Helpers.
 Require Import Relation_Operators.
+Require Import RelationClasses.
+Require Import Helpers.Instances.
 Require Import Compile.
 Require Import Equiv ProcMatch.
 
 Global Set Implicit Arguments.
 Global Generalizable All Variables.
 
+Section ExecOps.
+
+  Variable State:Type.
+  Variable opT:Type -> Type.
+  Variable op_step: OpSemantics opT State.
+
+  Definition exec_ops (s s' : State) : Prop :=
+    clos_refl_trans_1n _
+                       (fun s0 s1 =>
+                          exists tid `(op' : opT T') r' evs,
+                            op_step op' tid s0 r' s1 evs)
+                       s s'.
+
+  Lemma exec_ops_one : forall s s',
+      forall T (op: opT T) tid r evs,
+        op_step op tid s r s' evs ->
+        exec_ops s s'.
+  Proof.
+    unfold exec_ops; intros.
+    econstructor; [ | reflexivity ].
+    descend; eauto.
+  Qed.
+
+  Global Instance exec_ops_pre : PreOrder exec_ops.
+  Proof.
+    unfold exec_ops.
+    constructor; hnf; intros.
+    reflexivity.
+    etransitivity; eauto.
+  Qed.
+
+  Lemma exec_ops_reflexive : forall s,
+      exec_ops s s.
+  Proof.
+    reflexivity.
+  Qed.
+
+End ExecOps.
+
+Hint Resolve exec_ops_one.
+Hint Resolve exec_ops_reflexive.
 
 Section Protocol.
 
@@ -31,35 +74,78 @@ Section Protocol.
       op_allow op tid s /\
       lo_step op tid s r s' evs.
 
-  Inductive follows_protocol_proc (tid : nat) (s : State) :
+  Definition spawn_follows_protocol (follows_protocol_proc: nat -> State -> forall T (p: proc opT T), Prop) tid (s: State) T (p: proc _ T) :=
+    (forall tid',
+        tid <> tid' ->
+        forall s',
+          exec_ops restricted_step s s' ->
+          follows_protocol_proc tid' s' _ p).
+
+  Theorem spawn_follows_protocol_stable : forall follows_protocol_proc
+                                      tid s T (p: proc _ T) s'
+                                      tid' T' (op: opT T') r evs,
+      tid <> tid' ->
+      spawn_follows_protocol follows_protocol_proc tid s p ->
+      restricted_step op tid' s r s' evs ->
+      spawn_follows_protocol follows_protocol_proc tid s' p.
+  Proof.
+    unfold spawn_follows_protocol; intros.
+    eapply H0; eauto.
+    transitivity s'; eauto.
+  Qed.
+
+  Theorem follows_protocol_implies_spawn_follows_protocol_subset :
+    forall (follows_protocol_proc: nat -> State -> forall T (p: proc opT T), Prop)
+      tid s T (p: proc _ T),
+      (forall tid s, follows_protocol_proc tid s _ p) ->
+      spawn_follows_protocol follows_protocol_proc tid s p.
+  Proof.
+    unfold spawn_follows_protocol in *; intros.
+    eauto.
+  Qed.
+
+  Theorem spawn_follows_protocol_at_other_tid :
+    forall follows_protocol_proc
+      T (p: proc _ T) tid tid' s,
+      tid <> tid' ->
+      spawn_follows_protocol follows_protocol_proc tid s p ->
+      follows_protocol_proc tid' s _ p.
+  Proof.
+    unfold spawn_follows_protocol; intros.
+    eapply H0; eauto.
+  Qed.
+
+  Inductive follows_protocol_proc : forall (tid : nat) (s : State),
     forall T (p : proc opT T), Prop :=
   | FollowsProtocolProcOp :
-    forall T (op : opT T),
+    forall tid s T (op : opT T),
     op_allow op tid s ->
     follows_protocol_proc tid s (Op op)
   | FollowsProtocolProcBind :
-    forall T1 T2 (p1 : proc _ T1) (p2 : T1 -> proc _ T2),
+    forall tid s T1 T2 (p1 : proc _ T1) (p2 : T1 -> proc _ T2),
     follows_protocol_proc tid s p1 ->
     (forall r s',
       exec_any restricted_step tid s p1 r s' ->
       follows_protocol_proc tid s' (p2 r)) ->
     follows_protocol_proc tid s (Bind p1 p2)
   | FollowsProtocolProcUntil :
-    forall T (p : option T -> proc _ T) c v,
+    forall tid s T (p : option T -> proc _ T) c v,
     (forall s' v',
       follows_protocol_proc tid s' (p v')) ->
     follows_protocol_proc tid s (Until c p v)
   | FollowsProtocolProcRet :
-    forall T (v : T),
+    forall tid s T (v : T),
     follows_protocol_proc tid s (Ret v)
+  | FollowsProtocolProcSpawn :
+      forall tid s T (p: proc _ T),
+        spawn_follows_protocol follows_protocol_proc tid s p ->
+        follows_protocol_proc tid s (Spawn p)
   .
-
 
   Definition follows_protocol_s (ts : @threads_state opT) (s : State) :=
     forall tid T (p : proc _ T),
       ts [[ tid ]] = Proc p ->
       follows_protocol_proc tid s p.
-
 
   Variable allowed_stable :
     forall `(op : opT T) `(op' : opT T') tid tid' s s' r evs,
@@ -69,16 +155,16 @@ Section Protocol.
       op_allow op tid s'.
 
   Theorem follows_protocol_preserves_exec_tid' :
-    forall tid `(p : proc _ T) s s' result evs,
+    forall tid `(p : proc _ T) s s' result spawned evs,
       follows_protocol_proc tid s p ->
-      exec_tid lo_step tid s p s' result evs ->
-      exec_tid restricted_step tid s p s' result evs.
+      exec_tid lo_step tid s p s' result spawned evs ->
+      exec_tid restricted_step tid s p s' result spawned evs.
   Proof.
     intros.
     induction H0; simpl in *; intros; eauto;
       match goal with
       | H : follows_protocol_proc _ _ _ |- _ =>
-        inversion H; clear H; repeat sigT_eq; subst
+        invert H
       end; eauto.
     unfold restricted_step; eauto.
   Qed.
@@ -93,9 +179,9 @@ Section Protocol.
   Qed.
 
   Theorem exec_tid_restricted_to_nilpotent :
-    forall tid `(p : proc _ T) s s' result evs,
-      exec_tid restricted_step tid s p s' result evs ->
-      exec_tid nilpotent_step tid s p s' result evs.
+    forall tid `(p : proc _ T) s s' result spawned evs,
+      exec_tid restricted_step tid s p s' result spawned evs ->
+      exec_tid nilpotent_step tid s p s' result spawned evs.
   Proof.
     intros.
     induction H; simpl in *; intros; eauto.
@@ -105,10 +191,10 @@ Section Protocol.
   Qed.
 
   Theorem follows_protocol_preserves_exec_tid :
-    forall tid `(p : proc _ T) s s' result evs,
+    forall tid `(p : proc _ T) s s' result spawned evs,
       follows_protocol_proc tid s p ->
-      exec_tid lo_step tid s p s' result evs ->
-      exec_tid nilpotent_step tid s p s' result evs.
+      exec_tid lo_step tid s p s' result spawned evs ->
+      exec_tid nilpotent_step tid s p s' result spawned evs.
   Proof.
     intros.
     eapply exec_tid_restricted_to_nilpotent.
@@ -121,9 +207,9 @@ Section Protocol.
   Hint Constructors follows_protocol_proc.
 
   Theorem exec_tid_preserves_follows_protocol :
-    forall `(p : proc opT T) tid s s' p' evs,
+    forall `(p : proc opT T) tid s s' p' spawned evs,
     follows_protocol_proc tid s p ->
-    exec_tid lo_step tid s p s' (inr p') evs ->
+    exec_tid lo_step tid s p s' (inr p') spawned evs ->
     follows_protocol_proc tid s' p'.
   Proof.
     intros.
@@ -161,16 +247,19 @@ Section Protocol.
       follows_protocol_proc tid s' p.
   Proof.
     intros.
-    induction H0; eauto.
+    generalize dependent tid'.
+    induction H0; intros; eauto.
+    constructor; intros.
+    eauto using spawn_follows_protocol_stable.
   Qed.
 
   Hint Resolve follows_protocol_stable.
 
   Theorem exec_tid'_preserves_follows_protocol :
-    forall `(p : proc opT T) `(p' : proc opT T') tid tid' s s' r evs,
+    forall `(p : proc opT T) `(p' : proc opT T') tid tid' s s' r spawned evs,
       tid <> tid' ->
       follows_protocol_proc tid s p ->
-      exec_tid restricted_step tid' s p' s' r evs ->
+      exec_tid restricted_step tid' s p' s' r spawned evs ->
       no_atomics p' ->
       follows_protocol_proc tid s' p.
   Proof.
@@ -178,15 +267,15 @@ Section Protocol.
     induction H1; intros; simpl in *; try congruence;
       match goal with
       | H : no_atomics _ |- _ =>
-        inversion H; clear H; subst; repeat sigT_eq
+        invert H
       end; eauto.
   Qed.
 
   Theorem follows_protocol_s_exec_tid_upd :
-    forall ts tid `(p : proc _ T) s s' result evs,
+    forall ts tid `(p : proc _ T) s s' result spawned evs,
       follows_protocol_s ts s ->
       ts [[ tid ]] = Proc p ->
-      exec_tid lo_step tid s p s' result evs ->
+      exec_tid lo_step tid s p s' result spawned evs ->
       no_atomics_ts ts ->
       follows_protocol_s ts [[ tid := match result with
                                       | inl _ => NoProc
@@ -233,11 +322,15 @@ Section Protocol.
 
     clear dependent ts.
     generalize dependent s.
+    generalize dependent tid.
 
     match goal with
     | H : Compile.compile_ok _ _ _ |- _ =>
       induction H; intros; eauto
     end.
+
+    constructor.
+    eapply follows_protocol_implies_spawn_follows_protocol_subset; eauto.
   Qed.
 
 End Protocol.
