src/Helpers/Helpers.v
@@ -244,6 +244,8 @@ Ltac propositional :=
   repeat match goal with
          | |- forall _, _ => intros
          | [ H: _ /\ _ |- _ ] => destruct H
+         | [ H: False |- _ ] => solve [ destruct H ]
+         | [ H: True |- _ ] => clear H
          | [ H: ?P -> _, H': ?P |- _ ] =>
            match type of P with
            | Prop => specialize (H H')
@@ -258,6 +260,17 @@ Ltac propositional :=
          | [ H: ?P |- ?P ] => exact H
          | _ => progress subst
          end.
+
+(** prove_hyps on a hypothesis H of the form [P1 -> Pn -> Q] produces [P1] ...
+[Pn] as goals and changes [H] to [Q] *)
+Ltac prove_hyps H :=
+  match type of H with
+  | ?P -> ?Q => let HP := fresh in
+              assert P as HP;
+              [ | specialize (H HP); clear HP; prove_hyps H ]
+  | _ => idtac
+  end.
+
 
 (** * Instantiate existentials (deex) *)
 
