src/Helpers/Instances.v
@@ -1,0 +1,37 @@
+Require Import RelationClasses.
+Require Import Relation_Operators.
+Require Import Ordering.
+Require Import ProofIrrelevance.
+
+Require Import Helpers.Helpers.
+
+Local Hint Constructors clos_refl_trans_1n.
+Instance clos_rt1n_pre A (R: A -> A -> Prop) : PreOrder (clos_refl_trans_1n A R).
+Proof.
+  constructor; hnf; eauto.
+  induction 1; eauto.
+Qed.
+
+Instance comparison_eq_dec : EqualDec comparison.
+hnf; decide equality.
+Qed.
+
+Instance ord_eq_dec A {o:Ordering A} : EqualDec A.
+Proof.
+  hnf; intros.
+  destruct (cmp x y == Eq).
+  apply cmp_eq in e; auto.
+  right; intro; subst.
+  rewrite cmp_refl in n; congruence.
+Qed.
+
+Instance sigT_eq_dec A (P: A -> Prop) (dec:EqualDec A) : EqualDec (sig P).
+Proof.
+  hnf; intros.
+  destruct x as [x ?], y as [y ?].
+  destruct (x == y); subst; [ left | right ].
+  - f_equal.
+    apply proof_irrelevance.
+  - intro.
+    invert H; congruence.
+Qed.
