src/Spec/Trace.v
@@ -1,0 +1,44 @@
+Require Import Helpers.Helpers.
+
+Require List.
+Import List.ListNotations.
+Open Scope list.
+
+Set Implicit Arguments.
+
+Inductive event :=
+| Event : forall T (v : T), event.
+
+Inductive trace :=
+| TraceEvent : forall (tid : nat) (ev : event), trace -> trace
+| TraceEmpty : trace.
+
+
+Fixpoint prepend tid (evs : list event) (tr : trace) : trace :=
+  match evs with
+  | nil => tr
+  | e :: evs' =>
+    TraceEvent tid e (prepend tid evs' tr)
+  end.
+
+Theorem prepend_empty_eq : forall tid evs evs',
+    prepend tid evs TraceEmpty = prepend tid evs' TraceEmpty ->
+    evs = evs'.
+Proof.
+  intros.
+  generalize dependent evs'.
+  induct evs.
+  - destruct evs'; simpl in *; congruence.
+  - destruct evs'; simpl in *; try congruence.
+    invert H.
+    f_equal; eauto.
+Qed.
+
+Lemma prepend_app : forall `(evs1 : list event) evs2 tr tid,
+    prepend tid (evs1 ++ evs2) tr = prepend tid evs1 (prepend tid evs2 tr).
+Proof.
+  induction evs1; simpl; intros; eauto.
+  rewrite IHevs1; eauto.
+Qed.
+
+Arguments Event {T}.
